\begin{enumerate}
	\item $A:\R_+\times\R_+\rightarrow\R$, onde
	\[
		(x,y)\mapsto A(x,y)=xy
	\]
	e $P:\R_+\times\R_+\rightarrow\R$, onde
	\[
		(x,y)\mapsto P(x,y)=2x+y.
	\]

	\item Como $P(x,y)=2x+y=200$, então $y=200-2x$ e portanto podemos definir
	$a:[0,100]\rightarrow\R$ (pois $y$ tem que ser positivo) e
	\[
		a(x)=A(x,200-2x)=x(200-2x)=-2x^2+200x.
	\]

	\item Dessa vez, a partir de $2x+y=200$, tomamos $x=\frac{200-y}{2}$.
	Então definimos $b:[0,200]\rightarrow\R$ (pois $x$ tem que ser positivo) e
	\[
		b(y)=A(\frac{200-y}{2},y)=\frac{200-y}{2}y=\frac{200y-y^2}{2}.
	\]
\end{enumerate}
